crates/proof/host/src/bindings.rs
@@ -1950,6 +1950,56 @@ pub mod exports {
                 }
                 #[doc(hidden)]
                 #[allow(non_snake_case)]
+                pub unsafe fn _export_method_arena_ty_forall_cabi<T: GuestArena>(
+                    arg0: *mut u8,
+                    arg1: i64,
+                    arg2: i64,
+                ) -> *mut u8 {
+                    #[cfg(target_arch = "wasm32")] _rt::run_ctors_once();
+                    let result0 = T::ty_forall(
+                        unsafe { ArenaBorrow::lift(arg0 as u32 as usize) }.get(),
+                        arg1 as u64,
+                        arg2 as u64,
+                    );
+                    let ptr1 = (&raw mut _RET_AREA.0).cast::<u8>();
+                    match result0 {
+                        Ok(e) => {
+                            *ptr1.add(0).cast::<u8>() = (0i32) as u8;
+                            *ptr1.add(8).cast::<i64>() = _rt::as_i64(e);
+                        }
+                        Err(e) => {
+                            *ptr1.add(0).cast::<u8>() = (1i32) as u8;
+                            let vec2 = (e.into_bytes()).into_boxed_slice();
+                            let ptr2 = vec2.as_ptr().cast::<u8>();
+                            let len2 = vec2.len();
+                            ::core::mem::forget(vec2);
+                            *ptr1
+                                .add(8 + 1 * ::core::mem::size_of::<*const u8>())
+                                .cast::<usize>() = len2;
+                            *ptr1.add(8).cast::<*mut u8>() = ptr2.cast_mut();
+                        }
+                    };
+                    ptr1
+                }
+                #[doc(hidden)]
+                #[allow(non_snake_case)]
+                pub unsafe fn __post_return_method_arena_ty_forall<T: GuestArena>(
+                    arg0: *mut u8,
+                ) {
+                    let l0 = i32::from(*arg0.add(0).cast::<u8>());
+                    match l0 {
+                        0 => {}
+                        _ => {
+                            let l1 = *arg0.add(8).cast::<*mut u8>();
+                            let l2 = *arg0
+                                .add(8 + 1 * ::core::mem::size_of::<*const u8>())
+                                .cast::<usize>();
+                            _rt::cabi_dealloc(l1, l2, 1);
+                        }
+                    }
+                }
+                #[doc(hidden)]
+                #[allow(non_snake_case)]
                 pub unsafe fn _export_method_arena_model_cabi<T: GuestArena>(
                     arg0: *mut u8,
                     arg1: i64,
@@ -3558,6 +3608,56 @@ pub mod exports {
                 #[doc(hidden)]
                 #[allow(non_snake_case)]
                 pub unsafe fn __post_return_method_kernel_ty_exists<T: GuestKernel>(
+                    arg0: *mut u8,
+                ) {
+                    let l0 = i32::from(*arg0.add(0).cast::<u8>());
+                    match l0 {
+                        0 => {}
+                        _ => {
+                            let l1 = *arg0.add(8).cast::<*mut u8>();
+                            let l2 = *arg0
+                                .add(8 + 1 * ::core::mem::size_of::<*const u8>())
+                                .cast::<usize>();
+                            _rt::cabi_dealloc(l1, l2, 1);
+                        }
+                    }
+                }
+                #[doc(hidden)]
+                #[allow(non_snake_case)]
+                pub unsafe fn _export_method_kernel_ty_forall_cabi<T: GuestKernel>(
+                    arg0: *mut u8,
+                    arg1: i64,
+                    arg2: i64,
+                ) -> *mut u8 {
+                    #[cfg(target_arch = "wasm32")] _rt::run_ctors_once();
+                    let result0 = T::ty_forall(
+                        unsafe { KernelBorrow::lift(arg0 as u32 as usize) }.get(),
+                        arg1 as u64,
+                        arg2 as u64,
+                    );
+                    let ptr1 = (&raw mut _RET_AREA.0).cast::<u8>();
+                    match result0 {
+                        Ok(e) => {
+                            *ptr1.add(0).cast::<u8>() = (0i32) as u8;
+                            *ptr1.add(8).cast::<i64>() = _rt::as_i64(e);
+                        }
+                        Err(e) => {
+                            *ptr1.add(0).cast::<u8>() = (1i32) as u8;
+                            let vec2 = (e.into_bytes()).into_boxed_slice();
+                            let ptr2 = vec2.as_ptr().cast::<u8>();
+                            let len2 = vec2.len();
+                            ::core::mem::forget(vec2);
+                            *ptr1
+                                .add(8 + 1 * ::core::mem::size_of::<*const u8>())
+                                .cast::<usize>() = len2;
+                            *ptr1.add(8).cast::<*mut u8>() = ptr2.cast_mut();
+                        }
+                    };
+                    ptr1
+                }
+                #[doc(hidden)]
+                #[allow(non_snake_case)]
+                pub unsafe fn __post_return_method_kernel_ty_forall<T: GuestKernel>(
                     arg0: *mut u8,
                 ) {
                     let l0 = i32::from(*arg0.add(0).cast::<u8>());
@@ -6329,6 +6429,11 @@ pub mod exports {
                         name: u64,
                         predicate: u64,
                     ) -> Result<u64, _rt::String>;
+                    fn ty_forall(
+                        &self,
+                        name: u64,
+                        predicate: u64,
+                    ) -> Result<u64, _rt::String>;
                     fn model(
                         &self,
                         name: u64,
@@ -6514,6 +6619,11 @@ pub mod exports {
                     fn ty_lam(&self, binder: u64, body: u64) -> Result<u64, _rt::String>;
                     fn ty_fv(&self, name: u64, kind: u64) -> Result<u64, _rt::String>;
                     fn ty_exists(
+                        &self,
+                        name: u64,
+                        predicate: u64,
+                    ) -> Result<u64, _rt::String>;
+                    fn ty_forall(
                         &self,
                         name: u64,
                         predicate: u64,
@@ -7065,6 +7175,18 @@ pub mod exports {
                         mut u8,) { unsafe { $($path_to_types)*::
                         __post_return_method_arena_ty_exists::<<$ty as
                         $($path_to_types)*:: Guest >::Arena > (arg0) } } #[unsafe
+                        (export_name =
+                        "nucleus:proof/host@0.1.0#[method]arena.ty-forall")] unsafe
+                        extern "C" fn export_method_arena_ty_forall(arg0 : * mut u8, arg1
+                        : i64, arg2 : i64,) -> * mut u8 { unsafe { $($path_to_types)*::
+                        _export_method_arena_ty_forall_cabi::<<$ty as
+                        $($path_to_types)*:: Guest >::Arena > (arg0, arg1, arg2) } }
+                        #[unsafe (export_name =
+                        "cabi_post_nucleus:proof/host@0.1.0#[method]arena.ty-forall")]
+                        unsafe extern "C" fn _post_return_method_arena_ty_forall(arg0 : *
+                        mut u8,) { unsafe { $($path_to_types)*::
+                        __post_return_method_arena_ty_forall::<<$ty as
+                        $($path_to_types)*:: Guest >::Arena > (arg0) } } #[unsafe
                         (export_name = "nucleus:proof/host@0.1.0#[method]arena.model")]
                         unsafe extern "C" fn export_method_arena_model(arg0 : * mut u8,
                         arg1 : i64, arg2 : i64,) -> * mut u8 { unsafe {
@@ -7441,6 +7563,18 @@ pub mod exports {
                         unsafe extern "C" fn _post_return_method_kernel_ty_exists(arg0 :
                         * mut u8,) { unsafe { $($path_to_types)*::
                         __post_return_method_kernel_ty_exists::<<$ty as
+                        $($path_to_types)*:: Guest >::Kernel > (arg0) } } #[unsafe
+                        (export_name =
+                        "nucleus:proof/host@0.1.0#[method]kernel.ty-forall")] unsafe
+                        extern "C" fn export_method_kernel_ty_forall(arg0 : * mut u8,
+                        arg1 : i64, arg2 : i64,) -> * mut u8 { unsafe {
+                        $($path_to_types)*:: _export_method_kernel_ty_forall_cabi::<<$ty
+                        as $($path_to_types)*:: Guest >::Kernel > (arg0, arg1, arg2) } }
+                        #[unsafe (export_name =
+                        "cabi_post_nucleus:proof/host@0.1.0#[method]kernel.ty-forall")]
+                        unsafe extern "C" fn _post_return_method_kernel_ty_forall(arg0 :
+                        * mut u8,) { unsafe { $($path_to_types)*::
+                        __post_return_method_kernel_ty_forall::<<$ty as
                         $($path_to_types)*:: Guest >::Kernel > (arg0) } } #[unsafe
                         (export_name = "nucleus:proof/host@0.1.0#[method]kernel.model")]
                         unsafe extern "C" fn export_method_kernel_model(arg0 : * mut u8,
@@ -8193,12 +8327,14 @@ macro_rules! __export_kernel_host_impl {
 #[doc(inline)]
 pub(crate) use __export_kernel_host_impl as export;
 #[cfg(target_arch = "wasm32")]
-#[unsafe(link_section = "component-type:wit-bindgen:0.41.0:nucleus:proof@0.1.0:kernel-host:encoded world")]
+#[unsafe(
+    link_section = "component-type:wit-bindgen:0.41.0:nucleus:proof@0.1.0:kernel-host:encoded world"
+)]
 #[doc(hidden)]
 #[allow(clippy::octal_escapes)]
-pub static __WIT_BINDGEN_COMPONENT_TYPE: [u8; 6048] = *b"\
-\0asm\x0d\0\x01\0\0\x19\x16wit-component-encoding\x04\0\x07\x9e.\x01A\x02\x01A\x02\
-\x01B\xfa\x01\x01m\x03\x03syn\x05alpha\x04conv\x04\0\x07syn-rel\x03\0\0\x01m\x03\
+pub static __WIT_BINDGEN_COMPONENT_TYPE: [u8; 6105] = *b"\
+\0asm\x0d\0\x01\0\0\x19\x16wit-component-encoding\x04\0\x07\xd7.\x01A\x02\x01A\x02\
+\x01B\xfc\x01\x01m\x03\x03syn\x05alpha\x04conv\x04\0\x07syn-rel\x03\0\0\x01m\x03\
 \x04kind\x02ty\x02tm\x04\0\x04sort\x03\0\x02\x01r\x05\x0bexists-typew\x04bodyw\x0c\
 carrier-namew\x09base-namew\x07theoremw\x04\0\x0einfinity-axiom\x03\0\x04\x01r\x07\
 \x07carrierw\x09predicatew\x0bexists-typew\x0cpackage-bodyw\x0amodel-namew\x09ba\
@@ -8230,37 +8366,38 @@ a.to-cbor\x010\x01@\x01\x04self/\0\x0e\x04\0\x15[method]arena.address\x011\x01@\
 \0\x14[method]arena.ty-app\x016\x01@\x03\x04self/\x06binderw\x04bodyw\03\x04\0\x14\
 [method]arena.ty-lam\x017\x01@\x03\x04self/\x04namew\x04kindw\03\x04\0\x13[metho\
 d]arena.ty-fv\x018\x01@\x03\x04self/\x04namew\x09predicatew\03\x04\0\x17[method]\
-arena.ty-exists\x019\x04\0\x13[method]arena.model\x019\x01@\x03\x04self/\x04name\
-w\x02tyw\03\x04\0\x13[method]arena.tm-fv\x01:\x04\0\x11[method]arena.app\x016\x04\
-\0\x11[method]arena.lam\x017\x01@\x02\x04self/\x05value\x7f\03\x04\0\x16[method]\
-arena.bool-lit\x01;\x01@\x03\x04self/\x04leftw\x05rightw\03\x04\0\x13[method]are\
-na.tm-eq\x01<\x01@\x03\x04self/\x02tyw\x09predicatew\03\x04\0\x11[method]arena.e\
-ps\x01=\x01@\x03\x04self/\x06sourcew\x07foreignw\03\x04\0\x16[method]arena.kind-\
-ref\x01>\x04\0\x14[method]arena.ty-ref\x01>\x04\0\x14[method]arena.tm-ref\x01>\x04\
-\0\x19[method]arena.import-null\x014\x01@\x02\x04self/\x05value/\03\x04\0\x1a[me\
-thod]arena.import-arena\x01?\x01@\x02\x04self/\x07address\x0e\03\x04\0\x19[metho\
-d]arena.import-link\x01@\x01j\0\x01s\x01@\x02\x04self/\x0bpropositionw\0\xc1\0\x04\
-\0\x19[method]arena.add-context\x01B\x01@\x02\x04self/\x04names\x01\0\x04\0\x17[\
-method]arena.add-axiom\x01C\x01i\x0c\x01j\x01\xc4\0\x01s\x01@\x01\x05value/\0\xc5\
-\0\x04\0\x18[static]table.from-arena\x01F\x01@\x01\x05value\x1a\0\xc5\0\x04\0\x17\
-[static]table.from-blob\x01G\x01h\x0c\x01@\x01\x04self\xc8\0\0\x0e\x04\0\x15[met\
-hod]table.address\x01I\x01@\x01\x04self\xc8\0\0+\x04\0\x13[method]table.arena\x01\
-J\x01i\x0d\x01@\0\0\xcb\0\x04\0\x13[constructor]kernel\x01L\x01h\x0d\x01@\x01\x04\
-self\xcd\0\0+\x04\0\x14[method]kernel.arena\x01N\x01@\x01\x04self\xcd\0\0\x0e\x04\
-\0\x16[method]kernel.address\x01O\x01@\x01\x04self\xcd\0\0w\x04\0\x12[method]ker\
-nel.len\x01P\x01j\x01\x03\x01s\x01@\x02\x04self\xcd\0\x09referencew\0\xd1\0\x04\0\
-\x17[method]kernel.category\x01R\x01@\x02\x04self\xcd\0\x09referencew\03\x04\0\x19\
-[method]kernel.classifier\x01S\x04\0\x13[method]kernel.find\x01S\x04\0\x17[metho\
-d]kernel.find-mut\x01S\x01@\x03\x04self\xcd\0\x04leftw\x05rightw\0(\x04\0\x19[me\
-thod]kernel.equivalent\x01T\x04\0\x1d[method]kernel.equivalent-mut\x01T\x01@\x01\
-\x04self\xcd\0\03\x04\0\x18[method]kernel.kind-star\x01U\x01@\x03\x04self\xcd\0\x06\
-domainw\x08codomainw\03\x04\0\x17[method]kernel.kind-arr\x01V\x01@\x02\x04self\xcd\
-\0\x04starw\03\x04\0\x18[method]kernel.bool-type\x01W\x04\0\x15[method]kernel.ty\
--arr\x01V\x01@\x03\x04self\xcd\0\x08functionw\x08argumentw\03\x04\0\x15[method]k\
-ernel.ty-app\x01X\x01@\x03\x04self\xcd\0\x06binderw\x04bodyw\03\x04\0\x15[method\
-]kernel.ty-lam\x01Y\x01@\x03\x04self\xcd\0\x04namew\x04kindw\03\x04\0\x14[method\
-]kernel.ty-fv\x01Z\x01@\x03\x04self\xcd\0\x04namew\x09predicatew\03\x04\0\x18[me\
-thod]kernel.ty-exists\x01[\x04\0\x14[method]kernel.model\x01[\x01@\x03\x04self\xcd\
+arena.ty-exists\x019\x04\0\x17[method]arena.ty-forall\x019\x04\0\x13[method]aren\
+a.model\x019\x01@\x03\x04self/\x04namew\x02tyw\03\x04\0\x13[method]arena.tm-fv\x01\
+:\x04\0\x11[method]arena.app\x016\x04\0\x11[method]arena.lam\x017\x01@\x02\x04se\
+lf/\x05value\x7f\03\x04\0\x16[method]arena.bool-lit\x01;\x01@\x03\x04self/\x04le\
+ftw\x05rightw\03\x04\0\x13[method]arena.tm-eq\x01<\x01@\x03\x04self/\x02tyw\x09p\
+redicatew\03\x04\0\x11[method]arena.eps\x01=\x01@\x03\x04self/\x06sourcew\x07for\
+eignw\03\x04\0\x16[method]arena.kind-ref\x01>\x04\0\x14[method]arena.ty-ref\x01>\
+\x04\0\x14[method]arena.tm-ref\x01>\x04\0\x19[method]arena.import-null\x014\x01@\
+\x02\x04self/\x05value/\03\x04\0\x1a[method]arena.import-arena\x01?\x01@\x02\x04\
+self/\x07address\x0e\03\x04\0\x19[method]arena.import-link\x01@\x01j\0\x01s\x01@\
+\x02\x04self/\x0bpropositionw\0\xc1\0\x04\0\x19[method]arena.add-context\x01B\x01\
+@\x02\x04self/\x04names\x01\0\x04\0\x17[method]arena.add-axiom\x01C\x01i\x0c\x01\
+j\x01\xc4\0\x01s\x01@\x01\x05value/\0\xc5\0\x04\0\x18[static]table.from-arena\x01\
+F\x01@\x01\x05value\x1a\0\xc5\0\x04\0\x17[static]table.from-blob\x01G\x01h\x0c\x01\
+@\x01\x04self\xc8\0\0\x0e\x04\0\x15[method]table.address\x01I\x01@\x01\x04self\xc8\
+\0\0+\x04\0\x13[method]table.arena\x01J\x01i\x0d\x01@\0\0\xcb\0\x04\0\x13[constr\
+uctor]kernel\x01L\x01h\x0d\x01@\x01\x04self\xcd\0\0+\x04\0\x14[method]kernel.are\
+na\x01N\x01@\x01\x04self\xcd\0\0\x0e\x04\0\x16[method]kernel.address\x01O\x01@\x01\
+\x04self\xcd\0\0w\x04\0\x12[method]kernel.len\x01P\x01j\x01\x03\x01s\x01@\x02\x04\
+self\xcd\0\x09referencew\0\xd1\0\x04\0\x17[method]kernel.category\x01R\x01@\x02\x04\
+self\xcd\0\x09referencew\03\x04\0\x19[method]kernel.classifier\x01S\x04\0\x13[me\
+thod]kernel.find\x01S\x04\0\x17[method]kernel.find-mut\x01S\x01@\x03\x04self\xcd\
+\0\x04leftw\x05rightw\0(\x04\0\x19[method]kernel.equivalent\x01T\x04\0\x1d[metho\
+d]kernel.equivalent-mut\x01T\x01@\x01\x04self\xcd\0\03\x04\0\x18[method]kernel.k\
+ind-star\x01U\x01@\x03\x04self\xcd\0\x06domainw\x08codomainw\03\x04\0\x17[method\
+]kernel.kind-arr\x01V\x01@\x02\x04self\xcd\0\x04starw\03\x04\0\x18[method]kernel\
+.bool-type\x01W\x04\0\x15[method]kernel.ty-arr\x01V\x01@\x03\x04self\xcd\0\x08fu\
+nctionw\x08argumentw\03\x04\0\x15[method]kernel.ty-app\x01X\x01@\x03\x04self\xcd\
+\0\x06binderw\x04bodyw\03\x04\0\x15[method]kernel.ty-lam\x01Y\x01@\x03\x04self\xcd\
+\0\x04namew\x04kindw\03\x04\0\x14[method]kernel.ty-fv\x01Z\x01@\x03\x04self\xcd\0\
+\x04namew\x09predicatew\03\x04\0\x18[method]kernel.ty-exists\x01[\x04\0\x18[meth\
+od]kernel.ty-forall\x01[\x04\0\x14[method]kernel.model\x01[\x01@\x03\x04self\xcd\
 \0\x04namew\x02tyw\03\x04\0\x14[method]kernel.tm-fv\x01\\\x04\0\x12[method]kerne\
 l.app\x01X\x04\0\x12[method]kernel.lam\x01Y\x01@\x03\x04self\xcd\0\x09bool-typew\
 \x05value\x7f\03\x04\0\x17[method]kernel.bool-lit\x01]\x01@\x04\x04self\xcd\0\x09\
