lean/Nucleus/Nucleus/HolE/ClassicalEqTmSoundness.lean
@@ -66,16 +66,14 @@ structure ClassicalEqTmRuleLaws where
     CSemEq (Γ := Γ) x y (.sub A p) →
     CSemEq (Γ := Γ) (.rep A p x) (.rep A p y) A
   tyExists : ∀ {types depth} {Γ : BoundCtx ClassicalSig types depth}
-      {p q : Tm ClassicalSig (.star :: types) 0},
+      {p q : Tm ClassicalSig (.star :: types) depth},
     HasType Γ (.tyExists p) .boolTy → HasType Γ (.tyExists q) .boolTy →
-    CSemEq (Γ := (emptyBound : BoundCtx ClassicalSig (.star :: types) 0))
-      p q .boolTy →
+    CSemEq (Γ := weakenBoundCtx Γ) p q .boolTy →
     CSemEq (Γ := Γ) (.tyExists p) (.tyExists q) .boolTy
   tyForall : ∀ {types depth} {Γ : BoundCtx ClassicalSig types depth}
-      {p q : Tm ClassicalSig (.star :: types) 0},
+      {p q : Tm ClassicalSig (.star :: types) depth},
     HasType Γ (.tyForall p) .boolTy → HasType Γ (.tyForall q) .boolTy →
-    CSemEq (Γ := (emptyBound : BoundCtx ClassicalSig (.star :: types) 0))
-      p q .boolTy →
+    CSemEq (Γ := weakenBoundCtx Γ) p q .boolTy →
     CSemEq (Γ := Γ) (.tyForall p) (.tyForall q) .boolTy
   beta : ∀ {types depth} {Γ : BoundCtx ClassicalSig types depth}
       {A B : Ty ClassicalSig types} {body : Tm ClassicalSig types (depth + 1)}
